

Numerical Analysis Homework 3

Qiou Jiarui 3230103392 *

(信息与计算科学 2301), Zhejiang University

Due time: 2025 年 11 月 1 日

I. Natural Cubic Spline

At $x = 1$, the function value, first derivative, and second derivative must be continuous.

Let $p(x) = a + bx + cx^2 + dx^3$.

For the right segment $(2 - x)^3$ at $x = 1$:

$$q(1) = 1, \quad q'(1) = -3, \quad q''(1) = 6. \quad (1)$$

According to the continuity conditions, we have the following equations:

$$p(1) = a + b + c + d = 1, \quad (2)$$

$$p'(1) = b + 2c + 3d = -3, \quad (3)$$

$$p''(1) = 2c + 6d = 6. \quad (4)$$

Meanwhile, from $S(0) = 0$, we get

$$p(0) = a = 0. \quad (5)$$

From the above equations, we obtain:

$$p(x) = 12x - 18x^2 + 7x^3. \quad (6)$$

A natural cubic spline must satisfy $s''(0) = 0$ and $s''(2) = 0$.

$$p''(x) = -36 + 42x, \quad s''(0) = p''(0) = -36 \neq 0.$$

Therefore, $s(x)$ is not a natural cubic spline.

*Electronic address: 2222005915@qq.com

II. Quadratic Spline

II-a

A quadratic spline $s \in S_2^1$ is a quadratic polynomial on each subinterval $[x_i, x_{i+1}]$ and is globally C^1 continuous.

- Number of intervals: $n - 1$, total degrees of freedom: $3(n - 1)$.
- Constraints: n function value conditions, $n - 2$ internal first-derivative continuity conditions, giving a total of $2n - 2$ constraints.
- Remaining degrees of freedom: $3(n - 1) - (2n - 2) = n - 1$.

Hence, $n - 1$ additional conditions are required to uniquely determine the spline.

II-b

On each interval $[x_i, x_{i+1}]$, let

$$p_i(x) = A_i(x - x_i)^2 + B_i(x - x_i) + C_i. \quad (7)$$

From the conditions:

$$\begin{aligned} p_i(x_i) &= C_i = f_i, \\ p'_i(x_i) &= B_i = m_i, \\ p_i(x_{i+1}) &= A_i h_i^2 + m_i h_i + f_i = f_{i+1}, \quad h_i = x_{i+1} - x_i. \end{aligned}$$

We get

$$A_i = \frac{f_{i+1} - f_i - m_i h_i}{h_i^2}. \quad (8)$$

Thus,

$$p_i(x) = \frac{f_{i+1} - f_i - m_i h_i}{h_i^2} (x - x_i)^2 + m_i (x - x_i) + f_i. \quad (9)$$

II-c

At the node x_{i+1} , the first derivative is continuous:

$$p'_i(x_{i+1}) = p'_{i+1}(x_{i+1}) = m_{i+1}. \quad (10)$$

Compute

$$p'_i(x_{i+1}) = \frac{2(f_{i+1} - f_i)}{h_i} - m_i. \quad (11)$$

Hence, the recurrence formula is:

$$m_{i+1} = \frac{2(f_{i+1} - f_i)}{h_i} - m_i, \quad i = 1, 2, \dots, n - 2. \quad (12)$$

Given $m_1 = f'(a)$, we can successively compute m_2, m_3, \dots, m_{n-1} .

III. Natural Cubic Spline

Let

$$s_2(x) = a + bx + dx^2 + ex^3, \quad x \in [0, 1].$$

Apply continuity conditions at the node $x = 0$.

Function value continuity:

$$s_1(0) = s_2(0).$$

Compute

$$s_1(0) = 1 + c \cdot 1^3 = 1 + c, \quad s_2(0) = a.$$

Hence,

$$a = 1 + c. \quad (13)$$

First derivative continuity:

$$\begin{aligned} s'_1(x) &= 3c(x+1)^2, & s'_1(0) &= 3c, \\ s'_2(x) &= b + 2dx + 3ex^2, & s'_2(0) &= b. \end{aligned}$$

Therefore,

$$b = 3c. \quad (14)$$

Second derivative continuity:

$$\begin{aligned} s''_1(x) &= 6c(x+1), & s''_1(0) &= 6c, \\ s''_2(x) &= 2d + 6ex, & s''_2(0) &= 2d. \end{aligned}$$

Thus,

$$2d = 6c \quad \Rightarrow \quad d = 3c. \quad (15)$$

Natural boundary condition: at $x = 1$,

$$s''_2(1) = 0.$$

Compute

$$s''_2(1) = 2d + 6e = 0.$$

Substitute $d = 3c$ to obtain

$$2(3c) + 6e = 0 \Rightarrow 6c + 6e = 0.$$

Therefore,

$$e = -c. \quad (16)$$

Hence,

$$s_2(x) = (1 + c) + 3cx + 3cx^2 - cx^3.$$

Also, since $s(1) = -1$,

$$s_2(1) = 1 + c + 3c + 3c - c = 1 + 6c = -1.$$

Solve to get

$$6c = -2 \Rightarrow c = -\frac{1}{3}. \quad (17)$$

IV. Bending Energy

IV-a.

Given

$$f(x) = \cos\left(\frac{\pi}{2}x\right) \quad (18)$$

with nodes $-1, 0, 1$.

Let

$$s(x) = \begin{cases} s_1(x) = a_1 + b_1(x+1) + c_1(x+1)^2 + d_1(x+1)^3, & x \in [-1, 0], \\ s_2(x) = a_2 + b_2x + c_2x^2 + d_2x^3, & x \in [0, 1]. \end{cases} \quad (19)$$

From the function value conditions:

$$s_1(-1) = a_1 = 0, \quad (20)$$

$$s_1(0) = a_1 + b_1 + c_1 + d_1 = 1 \Rightarrow b_1 + c_1 + d_1 = 1, \quad (21)$$

$$s_2(0) = a_2 = 1, \quad (22)$$

$$s_2(1) = a_2 + b_2 + c_2 + d_2 = 0 \Rightarrow b_2 + c_2 + d_2 = -1. \quad (23)$$

First derivative continuity at $x = 0$:

$$s'_1(0) = b_1 + 2c_1 + 3d_1 = b_2 = s'_2(0). \quad (24)$$

Second derivative continuity at $x = 0$:

$$s''_1(0) = 2c_1 + 6d_1 = 2c_2 = s''_2(0). \quad (25)$$

Natural boundary conditions:

$$s_1''(-1) = 2c_1 = 0 \Rightarrow c_1 = 0, \quad (26)$$

$$s_2''(1) = 2c_2 + 6d_2 = 0 \Rightarrow c_2 + 3d_2 = 0. \quad (27)$$

Solving the system gives:

$$c_1 = 0, \quad d_1 = -\frac{1}{2}, \quad b_1 = \frac{3}{2}, \quad b_2 = 0, \quad c_2 = -\frac{3}{2}, \quad d_2 = \frac{1}{2}. \quad (28)$$

Hence,

$$s_1(x) = \frac{3}{2}(x+1) - \frac{1}{2}(x+1)^3, \quad (29)$$

$$s_2(x) = 1 - \frac{3}{2}x^2 + \frac{1}{2}x^3. \quad (30)$$

IV-b

The bending energy is defined as

$$E[g] = \int_{-1}^1 [g''(x)]^2 dx. \quad (31)$$

(i) Quadratic interpolation $g(x) = -x^2 + 1$:

$$g''(x) = -2, \quad E[g] = \int_{-1}^1 4 dx = 8. \quad (32)$$

(ii) The original function $f(x)$:

$$f''(x) = -\frac{\pi^2}{4} \cos\left(\frac{\pi}{2}x\right), \quad (33)$$

$$E[f] = \frac{\pi^4}{16} \int_{-1}^1 \cos^2\left(\frac{\pi}{2}x\right) dx = \frac{\pi^4}{16} \cdot 2 \cdot \frac{1}{2} \cdot 2 = \frac{\pi^4}{16} \approx 6.088. \quad (34)$$

(iii) Natural cubic spline $s(x)$:

On $[-1, 0]$, $s_1''(x) = -3(x+1)$; on $[0, 1]$, $s_2''(x) = -3+3x$.

$$E[s] = \int_{-1}^0 9(x+1)^2 dx + \int_0^1 9(1-x)^2 dx = 3 + 3 = 6. \quad (35)$$

Thus, $E[s] = 6$ is minimal, confirming that the natural cubic spline has the smallest bending energy.

V. Quadratic B-spline

V-a

The recursive definition of B-splines is given by:

$$B_i^0(x) = \begin{cases} 1, & x \in [t_i, t_{i+1}), \\ 0, & \text{otherwise.} \end{cases} \quad (36)$$

$$B_i^k(x) = \frac{x - t_i}{t_{i+k} - t_i} B_i^{k-1}(x) + \frac{t_{i+k+1} - x}{t_{i+k+1} - t_{i+1}} B_{i+1}^{k-1}(x). \quad (37)$$

For a quadratic B-spline $B_i^2(x)$, its support is $[t_{i-1}, t_{i+2}]$.

Let $h_1 = t_i - t_{i-1}$, $h_2 = t_{i+1} - t_i$, and $h_3 = t_{i+2} - t_{i+1}$.

The piecewise form is:

$$B_i^2(x) = \begin{cases} \frac{(x - t_{i-1})^2}{h_1(h_1 + h_2)}, & x \in [t_{i-1}, t_i), \\ \frac{x - t_{i-1}}{h_1 + h_2} \cdot \frac{t_{i+1} - x}{h_2} + \frac{t_{i+2} - x}{h_2 + h_3} \cdot \frac{x - t_i}{h_2}, & x \in [t_i, t_{i+1}), \\ \frac{(t_{i+2} - x)^2}{h_3(h_2 + h_3)}, & x \in [t_{i+1}, t_{i+2}), \\ 0, & \text{otherwise.} \end{cases} \quad (38)$$

For uniform knots $t_j = j$, i.e., $h_1 = h_2 = h_3 = 1$:

$$B_i^2(x) = \begin{cases} \frac{1}{2}(x - i + 1)^2, & x \in [i - 1, i), \\ \frac{1}{2} + (x - i) - (x - i)^2, & x \in [i, i + 1), \\ \frac{1}{2}(i + 2 - x)^2, & x \in [i + 1, i + 2), \\ 0, & \text{otherwise.} \end{cases} \quad (39)$$

V-b

Verification under uniform knots:

At $x = i$:

$$\frac{d}{dx} \left[\frac{1}{2}(x - i + 1)^2 \right] \Big|_{x=i} = 1, \quad (40)$$

$$\frac{d}{dx} \left[\frac{1}{2} + (x - i) - (x - i)^2 \right] \Big|_{x=i} = 1 - 2(x - i) \Big|_{x=i} = 1, \quad (41)$$

Hence, the derivative is continuous.

At $x = i + 1$:

$$\frac{d}{dx} \left[\frac{1}{2} + (x - i) - (x - i)^2 \right] \Big|_{x=i+1} = 1 - 2(1) = -1, \quad (42)$$

$$\frac{d}{dx} \left[\frac{1}{2}(i + 2 - x)^2 \right] \Big|_{x=i+1} = -(i + 2 - x) \Big|_{x=i+1} = -1, \quad (43)$$

Thus, the derivative is also continuous here.

For general (nonuniform) knots, the C^1 continuity is guaranteed by the general properties of B-splines.

V-c

For the middle interval $x \in [t_i, t_{i+1})$ under uniform knots:

$$B_i^2(x) = \frac{1}{2} + u - u^2, \quad u = x - i \in [0, 1), \quad (44)$$

$$\frac{d}{dx} B_i^2(x) = 1 - 2u = 0 \quad \Rightarrow \quad u = \frac{1}{2}, \quad (45)$$

Therefore,

$$x^* = i + \frac{1}{2}. \quad (46)$$

For general knots, the middle segment is a downward-opening quadratic function, hence there exists a unique maximum point.

V-d

Non-negativity is guaranteed by the definition of B-splines. The maximum occurs at the interior critical point; for uniform knots:

$$B_i^2(i + \frac{1}{2}) = \frac{1}{2} + \frac{1}{2} - \frac{1}{4} = \frac{3}{4} < 1, \quad (47)$$

and since the endpoint values are zero, we have $B_i^2(x) \in [0, \frac{3}{4}] \subset [0, 1)$.

V-e

The graph consists of three parabolic segments forming a bell-shaped curve:

- On $[i - 1, i)$: $\frac{1}{2}(x - i + 1)^2$, rising from 0 to 0.5;
- On $[i, i + 1)$: $\frac{1}{2} + (x - i) - (x - i)^2$, increasing from 0.5 to 0.75 and then decreasing back to 0.5;
- On $[i + 1, i + 2)$: $\frac{1}{2}(i + 2 - x)^2$, descending from 0.5 to 0.

The overall function is C^1 continuous, and the maximum value 0.75 occurs at $x = i + 0.5$.

VI. Verification of Theorem 3.32

Let $f_x(t) = (t - x)_+^2$. We verify the case of uniform knots $t_j = j$, where $a = i - 1$ and the nodes are $a, a + 1, a + 2, a + 3$.

Case 1: $x \in [a, a + 1)$

Let $u = x - a \in [0, 1)$.

Function values at the nodes:

$$\begin{aligned} f_x(a) &= 0, \\ f_x(a + 1) &= (1 - u)^2, \\ f_x(a + 2) &= (2 - u)^2, \\ f_x(a + 3) &= (3 - u)^2. \end{aligned}$$

First-order divided differences:

$$\begin{aligned}[a, a+1] &= (1-u)^2, \\ [a+1, a+2] &= (2-u)^2 - (1-u)^2 = 3-2u, \\ [a+2, a+3] &= (3-u)^2 - (2-u)^2 = 5-2u.\end{aligned}$$

Second-order divided differences:

$$\begin{aligned}[a, a+1, a+2] &= \frac{(3-2u) - (1-u)^2}{2} = \frac{2-u^2}{2}, \\ [a+1, a+2, a+3] &= \frac{(5-2u) - (3-2u)}{2} = 1.\end{aligned}$$

Third-order divided difference:

$$[a, a+1, a+2, a+3] = \frac{1 - \frac{2-u^2}{2}}{3} = \frac{u^2}{6}.$$

Multiplying by $t_{i+2} - t_{i-1} = 3$:

$$3 \cdot \frac{u^2}{6} = \frac{u^2}{2}.$$

Meanwhile, $B_i^2(x)$ in this interval equals $\frac{1}{2}(x - (i-1))^2 = \frac{1}{2}u^2$, which matches perfectly.

Other cases

Similar calculations verify that the equality also holds for $x \in [a+1, a+2)$ and $x \in [a+2, a+3)$, while both sides vanish outside the support.

Conclusion

The algebraic verification confirms that the theorem holds for $n = 2$.

VII. Scaled integral of B-splines.

We use the derivative formula for B-splines:

$$\frac{d}{dx} B_i^n(x) = \frac{n}{t_{i+n} - t_i} B_i^{n-1}(x) - \frac{n}{t_{i+n+1} - t_{i+1}} B_{i+1}^{n-1}(x). \quad (48)$$

Integrating over \mathbb{R} :

$$0 = \frac{n}{t_{i+n} - t_i} \int_{-\infty}^{\infty} B_i^{n-1}(x) dx - \frac{n}{t_{i+n+1} - t_{i+1}} \int_{-\infty}^{\infty} B_{i+1}^{n-1}(x) dx. \quad (49)$$

So

$$\frac{1}{t_{i+n} - t_i} \int_{-\infty}^{\infty} B_i^{n-1}(x) dx = \frac{1}{t_{i+n+1} - t_{i+1}} \int_{-\infty}^{\infty} B_{i+1}^{n-1}(x) dx. \quad (50)$$

Thus the quantity

$$Q_i^{n-1} := \frac{1}{t_{i+n} - t_i} \int_{-\infty}^{\infty} B_i^{n-1}(x) dx \quad (51)$$

is independent of i .

Now, it is known (and can be derived via recurrence from the above) that

$$\int_{-\infty}^{\infty} B_i^n(x) dx = \frac{t_{i+n+1} - t_i}{n+1}. \quad (52)$$

Therefore the scaled integral

$$S_i^n := \frac{\int_{-\infty}^{\infty} B_i^n(x) dx}{t_{i+n+1} - t_i} = \frac{1}{n+1} \quad (53)$$

is independent of i , regardless of knot spacing.

VIII. Symmetric Polynomials

Theorem:

$$h_m(x_1, \dots, x_n) = [x_1, \dots, x_n] t^{m+n-1}.$$

VIII-a

For $m = 4, n = 2$:

$$h_4(x_1, x_2) = [x_1, x_2] t^5. \quad (54)$$

By definition of divided difference:

$$[x_1, x_2] f = \frac{f(x_2) - f(x_1)}{x_2 - x_1}. \quad (55)$$

So

$$[x_1, x_2] t^5 = \frac{x_2^5 - x_1^5}{x_2 - x_1}. \quad (56)$$

Polynomial division:

$$x_2^5 - x_1^5 = (x_2 - x_1)(x_1^4 + x_1^3 x_2 + x_1^2 x_2^2 + x_1 x_2^3 + x_2^4). \quad (57)$$

Thus

$$[x_1, x_2] t^5 = x_1^4 + x_1^3 x_2 + x_1^2 x_2^2 + x_1 x_2^3 + x_2^4 = h_4(x_1, x_2). \quad (58)$$

Verified.

VIII-b

We prove:

$$h_m(x_1, \dots, x_n) = [x_1, \dots, x_n] t^{m+n-1}. \quad (59)$$

Base case $n = 1$:

$$[x_1] t^m = x_1^m = h_m(x_1). \quad (60)$$

Inductive step: Assume true for $n - 1$, i.e.

$$h_k(x_1, \dots, x_{n-1}) = [x_1, \dots, x_{n-1}] t^{k+n-2}. \quad (61)$$

$$h_k(x_2, \dots, x_n) = [x_2, \dots, x_n] t^{k+n-2}. \quad (62)$$

Now,

$$[x_1, \dots, x_n] t^{m+n-1} = \frac{[x_2, \dots, x_n] t^{m+n-1} - [x_1, \dots, x_{n-1}] t^{m+n-1}}{x_n - x_1}. \quad (63)$$

From the inductive assumption with $k = m + 1$:

$$[x_2, \dots, x_n] t^{m+n-1} = h_{m+1}(x_2, \dots, x_n), \quad (64)$$

$$[x_1, \dots, x_{n-1}] t^{m+n-1} = h_{m+1}(x_1, \dots, x_{n-1}). \quad (65)$$

So

$$[x_1, \dots, x_n] t^{m+n-1} = \frac{h_{m+1}(x_2, \dots, x_n) - h_{m+1}(x_1, \dots, x_{n-1})}{x_n - x_1}. \quad (66)$$

Using the known identity for complete symmetric polynomials:

$$h_{m+1}(x_2, \dots, x_n) - h_{m+1}(x_1, \dots, x_{n-1}) = (x_n - x_1) h_m(x_1, \dots, x_n). \quad (67)$$

Substitute:

$$[x_1, \dots, x_n] t^{m+n-1} = \frac{(x_n - x_1) h_m(x_1, \dots, x_n)}{x_n - x_1} = h_m(x_1, \dots, x_n). \quad (68)$$

Induction complete.